structure enhancement

lam_cl_es_no.v
@@ -8,7 +8,7 @@ Require Import reduction_semantics_facts.
 Open Scope list.
 
 
-Module Lam_ClES_NO_PreLang <: RED_SYNTAX.
+Module Lam_ClES_NO_RefLang <: REF_LANG.
 
   Require Export Peano_dec Compare_dec.
 
@@ -358,6 +358,21 @@ destruct t1, t2; destruct n0, n; autof ].
   Qed.
 
 
+  Lemma redex_trivial1 : forall {k} (r : redex k) ec t,
+                             ~dead_ckind (k+>ec) -> ec:[t] = r -> 
+                                 exists (v : value (k+>ec)), t = v.
+  Proof with auto.
+    intros k r ec t H H0.
+    destruct ec, r; destruct_all_CECa; inversion H0; subst;
+    solve 
+    [ eexists (vECaLam _); reflexivity
+    | eexists (vECaLam_cl _ _); reflexivity 
+    | match goal with H: _ (valCa_to_term0 ?v) = ?r |- _ => 
+          destruct v; inversion H 
+      end].
+  Qed.
+
+
   Lemma value_redex : forall {k} (v : value k) (r : redex k), 
                           value_to_term v <> redex_to_term r.
   Proof.
@@ -370,14 +385,40 @@ destruct t1, t2; destruct n0, n; autof ].
     end.
   Qed.
 
-End Lam_ClES_NO_PreLang.
+
+  Inductive decomp k : Set :=
+  | d_red : forall {k'}, redex k' -> context k k' -> decomp k
+  | d_val : value k -> decomp k.
+  Arguments d_val {k} _. Arguments d_red {k} {k'} _ _.
+
+  Definition decomp_to_term {k} (d : decomp k) :=
+      match d with
+      | d_val v     => value_to_term v
+      | d_red _ r c => c[r]
+      end.
+  Coercion decomp_to_term : decomp >-> term.
+
+
+
+  Definition immediate_subterm t0 t := exists ec, t = ec:[t0].
+
+  Lemma wf_immediate_subterm : well_founded immediate_subterm.
+  Proof. REF_LANG_Help.prove_st_wf. Qed.
+
+
+  Definition subterm_order := clos_trans_1n term immediate_subterm.
+  Notation "t1 <| t2" := (subterm_order t1 t2) (at level 70, no associativity).
+  Definition wf_subterm_order : well_founded subterm_order 
+      := wf_clos_trans_l _ _ wf_immediate_subterm.
+
+End Lam_ClES_NO_RefLang.
 
 
 
 
-Module Lam_ClES_NO_Strategy <: STRATEGY_STEP Lam_ClES_NO_PreLang.
+Module Lam_ClES_NO_Strategy <: REF_STRATEGY Lam_ClES_NO_RefLang.
 
-  Import Lam_ClES_NO_PreLang.
+  Import Lam_ClES_NO_RefLang.
 
 
   Inductive interm_dec k : Set :=
@@ -522,62 +563,10 @@ Module Lam_ClES_NO_Strategy <: STRATEGY_STEP Lam_ClES_NO_PreLang.
     solve [ autof ].
   Qed.
 
-End Lam_ClES_NO_Strategy.
 
 
 
-
-Module Lam_ClES_NO_Ref_minus <: RED_REF_LANG_minus.
-
-  Module SX := Lam_ClES_NO_PreLang.
-  Module ST := Lam_ClES_NO_Strategy.
-  Module RED_Props := Lam_ClES_NO_PreLang.
-
-  Export Lam_ClES_NO_PreLang Lam_ClES_NO_Strategy.
-
-
-  
-(*
-  Lemma dead_context_dead : 
-      forall {k1 k2}, context k1 k2 -> dead_ckind k1 -> dead_ckind k2.
-
-  Proof with auto.
-    intros ? ? c H; revert c.
-    induction 1.
-    - trivial.
-    - apply death_propagation...
-  Qed.*)
-
-
-
-  Lemma redex_trivial1 : forall {k} (r : redex k) ec t,
-                             ~dead_ckind (k+>ec) -> ec:[t] = r -> 
-                                 exists (v : value (k+>ec)), t = v.
-  Proof with auto.
-    intros k r ec t H H0.
-    destruct ec, r; destruct_all_CECa; inversion H0; subst;
-    solve 
-    [ eexists (vECaLam _); reflexivity
-    | eexists (vECaLam_cl _ _); reflexivity 
-    | match goal with H: _ (valCa_to_term0 ?v) = ?r |- _ => 
-          destruct v; inversion H 
-      end].
-  Qed.
-
-
-
-  Definition subterm_one_step t0 t := exists ec, t = ec:[t0].
-
-  Lemma wf_st1 : well_founded subterm_one_step.
-  Proof. RED_REF_LANG_Help.prove_st_wf. Qed.
-
-
-  Definition subterm_order := clos_trans_1n term subterm_one_step.
-  Notation "t1 <| t2" := (subterm_order t1 t2) (at level 40, no associativity).
-  Definition wf_sto : well_founded subterm_order := wf_clos_trans_l _ _ wf_st1.
-
-
-  Definition ec_order (k : ckind) (t : term) (ec ec0 : elem_context) : Prop :=
+  Definition search_order (k : ckind) (t : term) (ec ec0 : elem_context) : Prop :=
       match k with
       | CBot => False
       | _    => match ec, ec0 with 
@@ -585,15 +574,15 @@ Module Lam_ClES_NO_Ref_minus <: RED_REF_LANG_minus.
                 | _, _           => False
                 end
       end.
-  Notation "k , t |~  ec1 << ec2 " := (ec_order k t ec1 ec2) 
-               (at level 40, no associativity).
+  Notation "k , t |~  ec1 << ec2 " := (search_order k t ec1 ec2) 
+               (at level 70, no associativity).
 
 
-  Lemma wf_eco : forall k t, well_founded (ec_order k t).
-  Proof. RED_REF_LANG_Help.prove_ec_wf. Qed.
+  Lemma wf_search : forall k t, well_founded (search_order k t).
+  Proof. REF_LANG_Help.prove_ec_wf. Qed.
 
 
-  Lemma ec_order_antisym : forall k t ec ec0, 
+  Lemma search_order_antisym : forall k t ec ec0, 
       k, t |~ ec << ec0 -> ~ k, t |~ ec0 << ec.
 
   Proof.
@@ -603,7 +592,7 @@ Module Lam_ClES_NO_Ref_minus <: RED_REF_LANG_minus.
   Qed.
 
 
-  Lemma ec_order_trans :  forall k t ec0 ec1 ec2, 
+  Lemma search_order_trans :  forall k t ec0 ec1 ec2, 
       k,t |~ ec0 << ec1 -> k,t |~ ec1 << ec2 -> 
       k,t |~ ec0 << ec2.
 
@@ -614,7 +603,7 @@ Module Lam_ClES_NO_Ref_minus <: RED_REF_LANG_minus.
   Qed.
 
 
-  Lemma ec_order_comp_if : forall t ec0 ec1, 
+  Lemma search_order_comp_if : forall t ec0 ec1, 
       immediate_ec ec0 t -> immediate_ec ec1 t -> 
       forall k, ~ dead_ckind (k+>ec0) -> ~ dead_ckind (k+>ec1) ->
           k,t |~ ec0 << ec1 \/ k,t |~ ec1 << ec0 \/ ec0 = ec1.
@@ -635,7 +624,7 @@ Module Lam_ClES_NO_Ref_minus <: RED_REF_LANG_minus.
   Qed.
 
 
-  Lemma ec_order_comp_fi :
+  Lemma search_order_comp_fi :
       forall k t ec0 ec1,  k, t |~ ec0 << ec1 ->
           immediate_ec ec0 t /\ immediate_ec ec1 t /\ 
           ~ dead_ckind (k+>ec0) /\ ~ dead_ckind (k+>ec1).
@@ -650,15 +639,15 @@ Module Lam_ClES_NO_Ref_minus <: RED_REF_LANG_minus.
 
 
 
-  Definition only_empty t k := 
+(*  Definition only_empty t k := 
       forall t' {k'} (c : context k k'), c[t'] = t -> ~ dead_ckind k' -> 
           k = k' /\ c ~= [.](k).
 
   Definition only_trivial t k := 
       forall t' {k'} (c : context k k'),  c[t'] = t -> ~ dead_ckind k' -> 
-          k = k' /\ c ~= [.](k) \/ exists (v : value k'), t' = v.
+          k = k' /\ c ~= [.](k) \/ exists (v : value k'), t' = v.*)
 
-
+(*
   Lemma death_propagation2 : 
       forall k ec, ~ dead_ckind (k+>ec) -> ~ dead_ckind k.
 
@@ -667,48 +656,30 @@ Module Lam_ClES_NO_Ref_minus <: RED_REF_LANG_minus.
     apply H.
     apply death_propagation.
     assumption.
+  Qed.*)
+
+
+  Lemma dec_term_red_atom : 
+      forall t k {r : redex k}, dec_term t k = in_red r -> 
+          ~exists ec, immediate_ec ec t /\ ~dead_ckind (k+>ec).
+
+  Proof.
+    intros t k r H [ec [[t' H0] H1]]. 
+    destruct t, k, ec; 
+    inversion H0; subst; 
+    solve [autof].
   Qed.
 
 
-  Lemma dec_term_red_empty : 
-      forall t k (r : redex k), dec_term t k = in_red r -> only_empty t k.
+  Lemma dec_term_val_atom : 
+      forall t k {v : value k}, dec_term t k = in_val v -> 
+          ~exists ec, immediate_ec ec t /\ ~dead_ckind (k+>ec).
 
-  Proof with auto.
-    intros t k r H.
-    destruct t, k; destruct_all closure;
-    try match goal with t0 : term0 |- _ => destruct t0 end;
-    inversion H; subst; clear H;
-
-    try solve
-    [ intros t0 k' c H H0; generalize dependent t0;
-
-      induction c;
-      intros; simpl in *;
-      [ intuition
-      | destruct (IHc (death_propagation2 _ _ H0) _ H);
-        dep_subst;
-        destruct ec0;
-        solve [inversion H; auto] 
-    ] ].
-  Qed.
-
-
-  Lemma dec_term_val_empty : forall t k (v : value k), 
-                                 dec_term t k = in_val v -> only_empty t k.
-  Proof with auto.
-    intros t k v H.
-    destruct t;
-    intros t0 k' c' H0 H1; generalize dependent t0;
-    try solve
-    [ induction c';
-      intros t0 H0; simpl in *;
-      [ intuition
-      | destruct (IHc' (death_propagation2 _ _ H1) _ H0); dep_subst;
-        simpl in H;
-        destruct k2, ec0;
-        inversion H; subst; 
-        solve [discriminate H | autof] 
-    ] ].
+  Proof.
+    intros t k r H [ec [[t' H0] H1]]. 
+    destruct t, k, ec; 
+    inversion H0; subst; 
+    solve [autof].
   Qed.
 
 
@@ -734,7 +705,7 @@ Module Lam_ClES_NO_Ref_minus <: RED_REF_LANG_minus.
     [ autof
     | inversion H;
       intro G;
-      unfold ec_order in G; destruct G as (G, _);
+      unfold search_order in G; destruct G as (G, _);
       destruct G as (t1, G); inversion G; subst;
       destruct v0; 
       autof ].
@@ -783,7 +754,7 @@ Module Lam_ClES_NO_Ref_minus <: RED_REF_LANG_minus.
     subst.
 
     destruct k, ec0, ec'; autof;
-    unfold ec_order in H0; destruct H0 as (H, _);
+    unfold search_order in H0; destruct H0 as (H, _);
 
     try solve
     [ exists (vECaCa v);
@@ -792,26 +763,29 @@ Module Lam_ClES_NO_Ref_minus <: RED_REF_LANG_minus.
       trivial ].
   Qed.
 
-End Lam_ClES_NO_Ref_minus.
+End Lam_ClES_NO_Strategy.
 
 
 
-Module Lam_ClES_NO_Ref := mk_RedRefLang Lam_ClES_NO_Ref_minus.
-
+Module Lam_ClES_NO_Cal.
+  Module RefLang := Lam_ClES_NO_RefLang.
+  Module RefStrategy := Lam_ClES_NO_Strategy. 
+  Module RedLang := RedRefLang Lam_ClES_NO_RefLang RefStrategy.
+End Lam_ClES_NO_Cal.
 
 
 Require Import refocusing_semantics_derivation.
 Require Import refocusing_machine.
 
-Module Lam_ClES_NO_RefSem := RedRefSem Lam_ClES_NO_Ref.
-Module Lam_ClES_NO_EAM    := ProperEAMachine Lam_ClES_NO_Ref.R Lam_ClES_NO_RefSem.
+Module Lam_ClES_NO_RefSem := RedRefSem Lam_ClES_NO_Cal.
+Module Lam_ClES_NO_EAM    := ProperEAMachine Lam_ClES_NO_Cal.RedLang Lam_ClES_NO_RefSem.
 
 
 
 Module Lam_ClES_NO_EAM_safe <: AM_SAFE_REGION Lam_ClES_NO_EAM.
 
   Import Lam_ClES_NO_EAM.
-  Import Lam_ClES_NO_PreLang.
+  Import Lam_ClES_NO_RefLang.
 
 
 
@@ -960,7 +934,7 @@ End Lam_ClES_NO_EAM_safe.
 Module Lam_ClES_NO_EAM_minus <: DET_ABSTRACT_MACHINE.
 
   Module AM := Lam_ClES_NO_EAM.
-  Import Lam_ClES_NO_PreLang.
+  Import Lam_ClES_NO_RefLang.
 
   Definition term := term0.
   Definition value := AM.value.
