miniml.v
@@ -5,7 +5,7 @@ Require Import reduction_semantics_facts.
 
 
 
-Module MiniML_PreLang <: RED_SYNTAX.
+Module MiniML_RefLang <: REF_LANG.
 
   Parameter var : Set.
 
@@ -136,6 +136,7 @@ Module MiniML_PreLang <: RED_SYNTAX.
   Qed.
 
 
+
   Fixpoint compose {k1 k2} (c0 : context k1 k2) 
                       {k3} (c1 : context k3 k1) : context k3 k2 := 
       match c0 in context _ k2' return context k3 k2' with
@@ -207,14 +208,70 @@ Module MiniML_PreLang <: RED_SYNTAX.
       end.
   Notation contract' := (@contract ()).
 
-End MiniML_PreLang.
+
+  Lemma value_trivial1 : forall {k} (v : value k) ec t, 
+                             ~dead_ckind (k+>ec) -> ec:[t] = v ->
+                                 exists (v' : value (k+>ec)), t = v'.
+
+  Proof.
+    intros k v ec t H H0.
+    destruct ec, v; inversion H0; subst; 
+    eauto.
+  Qed.
+
+
+  Lemma value_redex : forall {k} (v : value k) (r : redex k), 
+                          value_to_term v <> redex_to_term r.
+  Proof.
+    destruct v; destruct r; intro H; discriminate H.
+  Qed.
+
+
+  Lemma redex_trivial1 : forall {k} (r : redex k) ec t,
+                             ~dead_ckind (k+>ec) -> ec:[t] = r -> 
+                                 exists (v : value (k+>ec)), t = v.
+  Proof with auto.
+    intros k r ec t H H0.
+    destruct ec, r; inversion H0; subst;
+    eauto.
+  Qed.
+
+
+
+  Definition immediate_subterm t0 t := exists ec, t = ec:[t0].
+
+  Lemma wf_immediate_subterm : well_founded immediate_subterm.
+  Proof. REF_LANG_Help.prove_st_wf. Qed.
+
+
+  Definition subterm_order := clos_trans_1n term immediate_subterm.
+  Notation "t1 <| t2" := (subterm_order t1 t2) (at level 70, no associativity).
+  Definition wf_subterm_order : well_founded subterm_order 
+      := wf_clos_trans_l _ _ wf_immediate_subterm.
+
+
+
+  Inductive decomp k : Set :=
+  | d_red : forall {k'}, redex k' -> context k k' -> decomp k
+  | d_val : value k -> decomp k.
+  Arguments d_val {k} _. Arguments d_red {k} {k'} _ _.
+
+  Definition decomp_to_term {k} (d : decomp k) :=
+      match d with
+      | d_val v     => value_to_term v
+      | d_red _ r c => c[r]
+      end.
+  Coercion decomp_to_term : decomp >-> term.
+  Notation decomp'   := (@decomp ()).
+
+End MiniML_RefLang.
 
 
 
 
-Module MiniML_Strategy <: STRATEGY_STEP MiniML_PreLang.
+Module MiniML_Strategy <: REF_STRATEGY MiniML_RefLang.
 
-  Import MiniML_PreLang.
+  Import MiniML_RefLang.
 
 
   Inductive interm_dec k : Set :=
@@ -310,98 +367,24 @@ Module MiniML_Strategy <: STRATEGY_STEP MiniML_PreLang.
 
   Proof. auto. Qed.
 
-End MiniML_Strategy.
 
 
 
-
-Module MiniML_Ref_minus <: RED_REF_LANG_minus.
-
-  Module SX := MiniML_PreLang.
-  Module ST := MiniML_Strategy.
-  Module RSF := RED_SYNTAX_Facts SX.
-  Export MiniML_PreLang MiniML_Strategy.
-  Import RSF.
-
-
-
-
-  Module RED_Props.
-
-    Include MiniML_PreLang.
-
-
-    Lemma value_trivial1 : forall {k} (v : value k) ec t, 
-                               ~dead_ckind (k+>ec) -> ec:[t] = v ->
-                                   exists (v' : value (k+>ec)), t = v'.
-
-    Proof.
-      intros k v ec t H H0.
-      destruct ec, v; inversion H0; subst; 
-      eauto.
-    Qed.
-
-
-    Lemma value_redex : forall {k} (v : value k) (r : redex k), 
-                            value_to_term v <> redex_to_term r.
-    Proof.
-      destruct v; destruct r; intro H; discriminate H.
-    Qed.
-
-  End RED_Props.
-
-
-
-
-  Lemma redex_trivial1 : forall {k} (r : redex k) ec t,
-                             ~dead_ckind (k+>ec) -> ec:[t] = r -> 
-                                 exists (v : value (k+>ec)), t = v.
-  Proof with auto.
-    intros k r ec t H H0.
-    destruct ec, r; inversion H0; subst;
-    eauto.
-  Qed.
-
-
-  Lemma dead_context_dead : 
-      forall {k1 k2}, context k1 k2 -> dead_ckind k1 -> dead_ckind k2.
-
-  Proof with auto.
-    intros ? ? c H; revert c.
-    induction 1.
-    - trivial.
-    - apply death_propagation...
-  Qed.
-
-
-
-
-  Definition subterm_one_step t0 t := exists ec, t = ec:[t0].
-
-  Lemma wf_st1 : well_founded subterm_one_step.
-  Proof. RED_REF_LANG_Help.prove_st_wf. Qed.
-
-
-  Definition subterm_order := clos_trans_1n term subterm_one_step.
-  Notation "t1 <| t2" := (subterm_order t1 t2) (at level 40, no associativity).
-  Definition wf_sto : well_founded subterm_order := wf_clos_trans_l _ _ wf_st1.
-
-
-  Definition ec_order (k : ckind) (t : term) (ec ec0 : elem_context) : Prop :=
+  Definition search_order (k : ckind) (t : term) (ec ec0 : elem_context) : Prop :=
       match ec, ec0 with
       | ap_l _,   ap_r _   => immediate_ec ec t /\ immediate_ec ec0 t
       | pair_l _, pair_r _ => immediate_ec ec t /\ immediate_ec ec0 t
       | _, _               => False
       end.
-  Notation "k , t |~  ec1 << ec2 " := (ec_order k t ec1 ec2) 
-               (at level 40, no associativity).
+  Notation "k , t |~  ec1 << ec2 " := (search_order k t ec1 ec2) 
+               (at level 70, no associativity).
 
 
-  Lemma wf_eco : forall k t, well_founded (ec_order k t).
-  Proof. RED_REF_LANG_Help.prove_ec_wf. Qed.
+  Lemma wf_search : forall k t, well_founded (search_order k t).
+  Proof. REF_LANG_Help.prove_ec_wf. Qed.
 
 
-  Lemma ec_order_antisym : forall k t ec ec0, 
+  Lemma search_order_antisym : forall k t ec ec0, 
       k, t |~ ec << ec0 -> ~ k, t |~ ec0 << ec.
   Proof.
     intros k ? ec ec0.
@@ -410,7 +393,7 @@ Module MiniML_Ref_minus <: RED_REF_LANG_minus.
   Qed.
 
 
-  Lemma ec_order_trans :  forall k t ec0 ec1 ec2, 
+  Lemma search_order_trans :  forall k t ec0 ec1 ec2, 
       k,t |~ ec0 << ec1 -> k,t |~ ec1 << ec2 -> 
       k,t |~ ec0 << ec2.
 
@@ -430,7 +413,7 @@ Module MiniML_Ref_minus <: RED_REF_LANG_minus.
 
 
 
-  Lemma ec_order_comp_if : forall t ec0 ec1, 
+  Lemma search_order_comp_if : forall t ec0 ec1, 
       immediate_ec ec0 t -> immediate_ec ec1 t -> 
       forall k, ~ dead_ckind (k+>ec0) -> ~ dead_ckind (k+>ec1) ->
           k,t |~ ec0 << ec1 \/ k,t |~ ec1 << ec0 \/ ec0 = ec1.
@@ -452,7 +435,7 @@ Module MiniML_Ref_minus <: RED_REF_LANG_minus.
   Qed.
 
 
-  Lemma ec_order_comp_fi :
+  Lemma search_order_comp_fi :
       forall k t ec0 ec1,  k, t |~ ec0 << ec1 ->
           immediate_ec ec0 t /\ immediate_ec ec1 t /\ 
           ~ dead_ckind (k+>ec0) /\ ~ dead_ckind (k+>ec1).
@@ -467,59 +450,37 @@ Module MiniML_Ref_minus <: RED_REF_LANG_minus.
 
 
 
-  Definition only_empty t k := 
+(*  Definition only_empty t k := 
       forall t' {k'} (c : context k k'), c[t'] = t -> ~ dead_ckind k' -> 
           k = k' /\ c ~= [.](k).
 
   Definition only_trivial t k := 
       forall t' {k'} (c : context k k'),  c[t'] = t -> ~ dead_ckind k' -> 
-          k = k' /\ c ~= [.](k) \/ exists (v : value k'), t' = v.
+          k = k' /\ c ~= [.](k) \/ exists (v : value k'), t' = v.*)
 
 
 
-  Lemma dec_term_red_empty : 
-      forall t {k} (r : redex k), dec_term t k = in_red r -> only_empty t k.
+  Lemma dec_term_red_atom : 
+      forall t k {r : redex k}, dec_term t k = in_red r -> 
+          ~exists ec, immediate_ec ec t /\ ~dead_ckind (k+>ec).
 
-  Proof with auto.
-    intros t k r H.
-
-    destruct t;
-        inversion H.
-
-    clear r H H1.
-
-    intros t0 k' c; generalize dependent t0.
-    induction c;
-        intros; simpl in *.
-    - intuition.
-    - destruct (IHc _ H) as (H1, H2)...
-      dep_subst.
-      solve [ destruct ec0; inversion H ].
+  Proof.
+    intros t k r H [ec [[t' H0] H1]]. 
+    destruct t, k, ec; 
+    inversion H0; subst; 
+    solve [autof].
   Qed.
 
 
-  Lemma dec_term_val_empty : 
-      forall t {k} (v : value k), dec_term t k = in_val v -> only_empty t k.
+  Lemma dec_term_val_atom : 
+      forall t k {v : value k}, dec_term t k = in_val v -> 
+          ~exists ec, immediate_ec ec t /\ ~dead_ckind (k+>ec).
 
   Proof.
-    intros t k v H.
-
-    destruct t;
-        inversion H;
-
-    solve 
-    [
-        clear v H H1;
-
-        intros t0 k' c; generalize dependent t0;
-        induction c;
-            intros; simpl in *;
-        solve
-        [ intuition
-        | destruct (IHc _ H) as (H1, H2); auto;
-          dep_subst;
-          destruct ec0; inversion H ]
-    ].
+    intros t k r H [ec [[t' H0] H1]]. 
+    destruct t, k, ec; 
+    inversion H0; subst; 
+    solve [autof].
   Qed.
 
 
@@ -596,30 +557,33 @@ Module MiniML_Ref_minus <: RED_REF_LANG_minus.
       eexists; trivial ].
   Qed.
 
-End MiniML_Ref_minus.
+End MiniML_Strategy.
 
 
 
+Module MiniML_Cal.
+  Module RefLang := MiniML_RefLang.
+  Module RefStrategy := MiniML_Strategy.
+  Module RedLang := RedRefLang RefLang RefStrategy.
 
-Module MiniML_Ref := mk_RedRefLang MiniML_Ref_minus.
+  (*Module Extras.
 
-Module MiniML_Extras.
+    Import MiniML_RefLang.
 
-  Import MiniML_Ref.R.
+    Notation context'  := (@context () ()).
+    Notation value'    := (@value ()).
+    Notation redex'    := (@redex ()).
+    Notation contract' := (@contract ()).
+    Notation decomp'   := (@decomp ()).
 
-  Notation context'  := (@context () ()).
-  Notation value'    := (@value ()).
-  Notation redex'    := (@redex ()).
-  Notation contract' := (@contract ()).
-  Notation decomp'   := (@decomp ()).
+  End Extras.*)
 
-End MiniML_Extras.
-
+End MiniML_Cal.
 
 
 
 Require Import refocusing_semantics_derivation.
 Require Import refocusing_machine.
 
-Module MiniML_RefSem := RedRefSem MiniML_Ref.
-Module MiniML_EAM    := ProperEAMachine MiniML_Ref.R MiniML_RefSem.
+Module MiniML_RefSem := RedRefSem MiniML_Cal.
+Module MiniML_EAM    := ProperEAMachine MiniML_Cal.RedLang MiniML_RefSem.
