refocusing_lang.v
@@ -2,16 +2,15 @@ Require Import Program.
 Require Import Util.
 Require Export reduction_semantics.
 Require Import reduction_semantics_facts.
-Require Export strategy_step.
+Require Export reduction_strategy.
 
 
 
 
-Module Type RED_REF_LANG.
+Module Type REF_LANG <: RED_STRATEGY_LANG.
 
-  Declare Module R  : RED_LANG.
-  Declare Module ST : STRATEGY_STEP R.
-  Export R ST.
+  Include RED_STRATEGY_LANG.
+
 
 
   (* A property of deterministic reduction semantics: *)
@@ -20,347 +19,130 @@ Module Type RED_REF_LANG.
                                  exists (v : value (k+>ec)), t = v.
 
 
-  Definition subterm_one_step t0 t := exists ec, t = ec:[t0].
-  Axiom wf_st1 : well_founded subterm_one_step.
+  Definition immediate_subterm t0 t := exists ec, t = ec:[t0].
+  Axiom wf_immediate_subterm : well_founded immediate_subterm.
 
 
-  Definition subterm_order := clos_trans_1n term subterm_one_step.
+  Definition subterm_order := clos_trans_1n term immediate_subterm.
   Notation "t1 <| t2" := (subterm_order t1 t2) (at level 70, no associativity).
-  Definition wf_sto : well_founded subterm_order
+  Definition wf_subterm_order : well_founded subterm_order
+      := wf_clos_trans_l _ _ wf_immediate_subterm.
 
-             := wf_clos_trans_l _ _ wf_st1.
+
+  Parameter contract : forall {k}, redex k -> option term.
+
+End REF_LANG.
 
 
-  Parameter ec_order : ckind -> term -> elem_context -> elem_context -> Prop.
-  Notation "k , t |~  ec1 << ec2 " := (ec_order k t ec1 ec2) 
-               (at level 70, t, ec1, ec2 at level 50, no associativity).
-  Axiom wf_eco : forall k t, well_founded (ec_order k t).
 
-  Axiom ec_order_antisym : forall k t ec ec0, 
+
+Module Type REF_STRATEGY (R : REF_LANG) <: RED_STRATEGY R.
+
+  Import R.
+
+  Include RED_STRATEGY R.
+
+
+
+  Axiom wf_search : forall k t, well_founded (search_order k t).
+
+  Axiom search_order_antisym : forall k t ec ec0, 
       k, t |~ ec << ec0 -> ~ k, t |~ ec0 << ec.
 
-  Axiom ec_order_trans   : forall k t ec0 ec1 ec2,
+  Axiom search_order_trans   : forall k t ec0 ec1 ec2,
       k, t |~ ec0 << ec1 -> k, t |~ ec1 << ec2 -> k,t |~ ec0 << ec2.
 
-  Axiom ec_order_comp_if : 
+  Axiom search_order_comp_if : 
       forall t ec0 ec1, immediate_ec ec0 t -> immediate_ec ec1 t -> 
           forall k, ~ dead_ckind (k+>ec0) -> ~ dead_ckind (k+>ec1) ->
               k, t |~ ec0 << ec1  \/  k, t |~ ec1 << ec0  \/  ec0 = ec1.
 
-  Axiom ec_order_comp_fi : forall k t ec0 ec1,
-      k, t |~ ec0 << ec1  ->  immediate_ec ec0 t /\ immediate_ec ec1 t /\ 
-                                  ~ dead_ckind (k+>ec0) /\ ~ dead_ckind (k+>ec1).
+  Axiom search_order_comp_fi : 
+      forall k t ec0 ec1,  k, t |~ ec0 << ec1 ->  
+          immediate_ec ec0 t /\ immediate_ec ec1 t /\ 
+              ~ dead_ckind (k+>ec0) /\ ~ dead_ckind (k+>ec1).
 
-  Definition only_empty t k :=
-      forall t' {k'} (c : context k k'), c[t'] = t -> ~ dead_ckind k' -> 
-          k = k' /\ c ~= [.](k).
+End REF_STRATEGY.
 
-  Definition only_trivial t k :=
-      forall t' {k'} (c : context k k'), c[t'] = t -> ~ dead_ckind k' -> 
-          k = k' /\ c ~= [.](k) \/ exists (v : value k'), t' = v.
 
-  Axiom dec_term_red_empty : 
-      forall t k {r : redex k}, dec_term t k = in_red r -> only_empty t k.
 
-  Axiom dec_term_val_empty : 
-      forall t k {v : value k}, dec_term t k = in_val v -> only_empty t k.
 
-  Axiom dec_term_term_top : 
-      forall t k {t' ec}, dec_term t k = in_term t' ec -> 
-          forall ec',  ~ k, t |~ ec << ec'.
+Module RedRefLang (R : REF_LANG) (ST : REF_STRATEGY R) <: RED_LANG.
 
-  Axiom dec_context_red_bot : 
-      forall k ec v {r : redex k}, dec_context ec k v = in_red r -> 
-          forall ec',  ~ k, ec:[v] |~ ec' << ec.
+  Module RF := RED_LANG_Facts R.
 
-  Axiom dec_context_val_bot : 
-      forall k ec v {v' : value k}, dec_context ec k v = in_val v' -> 
-          forall ec',  ~ k, ec:[v] |~ ec' << ec.
+  Include R.
+  Import ST RF.
 
-  Axiom dec_context_term_next : 
-      forall ec0 k v {t ec1}, dec_context ec0 k v = in_term t ec1 -> 
-      (*1*) k, ec0:[v] |~ ec1 << ec0 /\ 
-      (*2*) forall ec,  k, ec0:[v] |~ ec << ec0  ->  ~ k, ec0:[v] |~ ec1 << ec.
 
 
-  Axiom elem_context_det : 
-      forall t ec {t'}, t = ec:[t'] -> 
-          forall k ec',  k, t |~ ec' << ec -> 
-              exists (v : value (k+>ec)), t' = v.
+  Lemma decompose : 
+      forall (t : term) k1, ~ dead_ckind k1 ->
+          (exists (v : value k1), t = v) \/
+          (exists k2 (r : redex k2) (c : context k1 k2), t = c[r : term]).
 
-End RED_REF_LANG.
+  Proof with eauto.
+    induction t using (well_founded_ind wf_subterm_order); intros.
 
+    remember (dec_term t k1); assert (hh := dec_term_correct t k1);
+    symmetry in Heqi;
+    destruct i; rewrite Heqi in hh.
 
+    - right; exists k1; exists r; eexists [.]...
 
+    - destruct (H t0) with (k1 := k1+>e) as [(v, Hv) | (k2, (r, (c, Hrc)))].
+          repeat econstructor...
+          eapply dec_term_next_alive... 
 
-  Module Type __SIG1 (SX : RED_SYNTAX).
+      + { subst t0.
+        assert (~ dead_ckind (k1+>e)) as Hndk.
+          { eapply dec_term_next_alive... } 
+        clear Heqi; generalize dependent v.
+        induction e using (well_founded_ind (wf_search k1 t)); intros.
 
-    Import SX.
+        remember (dec_context e _ v); assert (ht := dec_context_correct e _ v); 
+        destruct i; rewrite <- Heqi in ht; try 
+        (   compute in hh; rewrite <- hh in ht).
 
-    Parameter init_ckind : ckind.
+        - right; exists k1; exists r; eexists [.]...
 
-    Axiom value_trivial1 : forall {k} (v : value k) ec t, 
-                               ~dead_ckind (k+>ec) -> ec:[t] = v -> 
-                                   exists (v' : value (k+>ec)), t = v'.
-    Axiom value_redex    : forall {k} (v : value k) (r : redex k), 
-                               value_to_term v <> redex_to_term r.
+        - destruct (H t0) with (k1 := k1+>e0) as [(v0, Hv) | (k2, (r, (c, Hrc)))].
+              repeat econstructor...
+              eapply dec_context_next_alive...
 
-    Parameter contract : forall {k}, redex k -> option term.
+          + symmetry in Heqi.
+            destruct (dec_context_term_next _ _ _ Heqi) as (H2, _).
 
-  End __SIG1.
+            subst t0.
+            assert (~ dead_ckind (k1+>e0)) as Hndk2.
+              { eapply dec_context_next_alive... }
+            rewrite <- hh in H2.
+            destruct (H1 e0 H2 Hndk2 v0 ht) as [(v1, Hv1) | (k2, (r, (c, Hrc)))].
+            * left; exists v1...
+            * right; exists k2; exists r; exists c...
 
+          + right; exists k2; exists r; exists (c~+e0=:[.]).
+            subst t0; rewrite plug_compose...
 
-Module Type RED_REF_LANG_minus.
+        - left; exists v0...
 
-  Declare Module SX : RED_SYNTAX.
-  Declare Module ST : STRATEGY_STEP SX.
-  Export SX ST.
-  Declare Module RED_Props : __SIG1 SX.
+        - intuition. 
+        }
 
+      + right; exists k2; exists r; exists (c~+(e=:[.])).
+        subst t0; rewrite plug_compose...
 
+    - left; exists v...
 
-    Axiom redex_trivial1 : forall {k} (r : redex k) ec t, 
-                               ~dead_ckind (k+>ec) -> ec:[t] = r -> 
-                                   exists (v : value (k+>ec)), t = v.
+    - intuition.
+  Qed.
 
+End RedRefLang.
 
 
 
-  Definition subterm_one_step t0 t := exists ec, t = ec:[t0].
-  Axiom wf_st1 : well_founded subterm_one_step.
 
-
-  Definition subterm_order := clos_trans_1n term subterm_one_step.
-  Notation "t1 <| t2" := (subterm_order t1 t2) (at level 70, no associativity).
-  Definition wf_sto : well_founded subterm_order := wf_clos_trans_l _ _ wf_st1.
-
-
-  Parameter ec_order : ckind -> term -> elem_context -> elem_context -> Prop.
-  Notation "k , t |~  ec1 << ec2 " := (ec_order k t ec1 ec2) 
-               (at level 70, t, ec1, ec2 at level 50, no associativity).
-  Axiom wf_eco : forall k t, well_founded (ec_order k t).
-
-  Axiom ec_order_antisym : forall k t ec ec0, 
-      k, t |~ ec << ec0 -> ~ k, t |~ ec0 << ec.
-
-  Axiom ec_order_trans   : forall k t ec0 ec1 ec2,
-      k, t |~ ec0 << ec1 -> k, t |~ ec1 << ec2 -> k,t |~ ec0 << ec2.
-
-  Axiom ec_order_comp_if : forall t ec0 ec1,
-      immediate_ec ec0 t -> immediate_ec ec1 t -> 
-      forall k, ~ dead_ckind (k+>ec0) -> ~ dead_ckind (k+>ec1) ->
-          k, t |~ ec0 << ec1  \/  k, t |~ ec1 << ec0  \/  ec0 = ec1.
-
-  Axiom ec_order_comp_fi : forall k t ec0 ec1,
-      k, t |~ ec0 << ec1  ->  immediate_ec ec0 t /\ immediate_ec ec1 t /\ 
-                                  ~ dead_ckind (k+>ec0) /\ ~ dead_ckind (k+>ec1).
-
-
-
-    Definition only_empty t k :=
-        forall t' {k'} (c : context k k'), c[t'] = t -> ~ dead_ckind k' -> 
-            k = k' /\ c ~= [.](k).
-    Definition only_trivial t k :=
-        forall t' {k'} (c : context k k'), c[t'] = t -> ~ dead_ckind k' -> 
-            k = k' /\ c ~= [.](k) \/ exists (v : value k'), t' = v.
-
-  Axiom dec_term_red_empty : 
-      forall t k {r : redex k}, dec_term t k = in_red r -> only_empty t k.
-
-  Axiom dec_term_val_empty : 
-      forall t k {v : value k}, dec_term t k = in_val v -> only_empty t k.
-
-  Axiom dec_term_term_top : 
-      forall t k {t' ec}, dec_term t k = in_term t' ec -> 
-          forall ec',  ~ k, t |~ ec << ec'.
-
-  Axiom dec_context_red_bot : 
-      forall k ec v {r : redex k}, dec_context ec k v = in_red r -> 
-          forall ec',  ~ k, ec:[v] |~ ec' << ec.
-
-  Axiom dec_context_val_bot : 
-      forall k ec v {v' : value k}, dec_context ec k v = in_val v' -> 
-          forall ec',  ~ k, ec:[v] |~ ec' << ec.
-
-  Axiom dec_context_term_next : 
-      forall ec0 k v {t ec1}, dec_context ec0 k v = in_term t ec1 -> 
-      (*1*) k, ec0:[v] |~ ec1 << ec0 /\ 
-      (*2*) forall ec,  k, ec0:[v] |~ ec << ec0  ->  ~ k, ec0:[v] |~ ec1 << ec.
-
-
-  Axiom elem_context_det : 
-      forall t ec {t'}, t = ec:[t'] -> 
-          forall k ec',  k, t |~ ec' << ec -> 
-              exists (v : value (k+>ec)), t' = v.
-
-End RED_REF_LANG_minus.
-
-
-
-
-Module mk_RedRefLang (PR : RED_REF_LANG_minus) <: RED_REF_LANG.
-
-  Module SXF := RED_SYNTAX_Facts PR.SX.
-  Import SXF.
-
-
-  Module R <: RED_LANG.
-
-    Include PR.SX.
-    Include PR.RED_Props.
-
-(*
-    Definition only_empty t k :=
-        forall t' {k'} (c : context k k'), c[t'] = t -> ~ dead_ckind k' -> 
-            k = k' /\ c ~= [.](k).
-    Definition only_trivial t k :=
-        forall t' {k'} (c : context k k'), c[t'] = t -> ~ dead_ckind k' -> 
-            k = k' /\ c ~= [.](k) \/ exists (v : value k'), t' = v.*)
-(*
-    Definition value_trivial1 : 
-        forall {k} (v : value k) ec t, 
-            ~dead_ckind (k+>ec) -> ec:[t] = v -> 
-                exists (v' : value (k+>ec)), t = v'
-
-        := @PR.RED_Props.value_trivial1.
-
-    Definition value_redex   : forall {k} (v : value k) (r : redex k), 
-                            value_to_term v <> redex_to_term r
-        := @PR.RED_Props.value_redex.*)
-
-
-    Lemma decompose : 
-        forall (t : term) k1, ~ dead_ckind k1 ->
-            (exists (v : value k1), t = v) \/
-            (exists k2 (r : redex k2) (c : context k1 k2), t = c[r]).
-
-    Proof with eauto.
-      induction t using (well_founded_ind PR.wf_sto); intros.
-
-      remember (PR.ST.dec_term t k1); assert (hh := PR.ST.dec_term_correct t k1);
-      symmetry in Heqi;
-      destruct i; rewrite Heqi in hh.
-
-      - right; exists k1; exists r; eexists [.]...
-
-      - destruct (H t0) with (k1 := k1+>e) as [(v, Hv) | (k2, (r, (c, Hrc)))].
-            repeat econstructor...
-            eapply PR.ST.dec_term_next_alive... 
-
-        + { subst t0.
-          assert (~ dead_ckind (k1+>e)) as Hndk.
-            { eapply PR.ST.dec_term_next_alive... } 
-          clear Heqi; generalize dependent v.
-          induction e using (well_founded_ind (PR.wf_eco k1 t)); intros.
-
-          remember (PR.ST.dec_context e _ v); assert (ht := PR.ST.dec_context_correct e _ v); 
-          destruct i; rewrite <- Heqi in ht; try 
-          (   compute in hh; rewrite <- hh in ht).
-
-          - right; exists k1; exists r; eexists [.]...
-
-          - destruct (H t0) with (k1 := k1+>e0) as [(v0, Hv) | (k2, (r, (c, Hrc)))].
-                repeat econstructor...
-                eapply PR.ST.dec_context_next_alive...
-
-            + symmetry in Heqi.
-              destruct (PR.dec_context_term_next _ _ _ Heqi) as (H2, _).
-
-              subst t0.
-              assert (~ dead_ckind (k1+>e0)) as Hndk2.
-                { eapply PR.ST.dec_context_next_alive... }
-              rewrite <- hh in H2.
-              destruct (H1 e0 H2 Hndk2 v0 ht) as [(v1, Hv1) | (k2, (r, (c, Hrc)))].
-              * left; exists v1...
-              * right; exists k2; exists r; exists c...
-
-            + right; exists k2; exists r; exists (c~+e0=:[.]).
-              subst t0; rewrite plug_compose...
-
-          - left; exists v0...
-
-          - intuition. 
-          }
-
-        + right; exists k2; exists r; exists (c~+(e=:[.])).
-          subst t0; rewrite plug_compose...
-
-      - left; exists v...
-
-      - intuition.
-    Qed. 
-
-(*
-    Definition init_ckind := PR.RED_Props.init_ckind.
-
-    Definition contract := @PR.RED_Props.contract.
-    Arguments contract {k} _.*)
-
-
-    Inductive decomp k : Set :=
-    | d_red : forall {k'}, redex k' -> context k k' -> decomp k
-    | d_val : value k -> decomp k.
-    Arguments d_val {k} _. Arguments d_red {k} {k'} _ _.
-
-
-    Definition decomp_to_term {k} (d : decomp k) :=
-        match d with
-        | d_val v     => value_to_term v
-        | d_red _ r c => c[r]
-        end.
-    Coercion decomp_to_term : decomp >-> term.
-
-  End R.
-
-  Export R.
-
-
-  Include PR.
-
-(*
-  Module ST := PR.ST.
-
-  Export R ST.
-
-
-  Definition redex_trivial1 {k} := @PR.redex_trivial1 k.
-
-  Definition subterm_one_step t0 t := exists ec, t = ec:[t0].
-  Definition wf_st1 := PR.wf_st1.
-
-
-  Definition subterm_order := clos_trans_1n term subterm_one_step.
-  Notation "t1 <| t2" := (subterm_order t1 t2) (at level 70, no associativity).
-  Definition wf_sto := wf_clos_trans_l _ _ wf_st1.
-
-
-  Definition ec_order := PR.ec_order.
-  Notation "k , t |~  ec1 << ec2 " := (ec_order k t ec1 ec2) 
-               (at level 70, t, ec1, ec2 at level 50, no associativity).
-  Definition wf_eco := PR.wf_eco.
-
-  Definition ec_order_antisym := PR.ec_order_antisym.
-  Definition ec_order_trans   := PR.ec_order_trans.
-  Definition ec_order_comp_if := PR.ec_order_comp_if.
-  Definition ec_order_comp_fi := PR.ec_order_comp_fi.
-
-
-  Definition dec_term_red_empty := PR.dec_term_red_empty.
-  Definition dec_term_val_empty := PR.dec_term_val_empty.
-  Definition dec_term_term_top  := PR.dec_term_term_top.
-
-  Definition dec_context_red_bot   := PR.dec_context_red_bot.
-  Definition dec_context_val_bot   := PR.dec_context_val_bot.
-  Definition dec_context_term_next := PR.dec_context_term_next.
-
-
-  Definition elem_context_det := PR.elem_context_det.*)
-
-End mk_RedRefLang.
-
-
-
-Module RED_REF_LANG_Help.
+Module REF_LANG_Help.
 
   Ltac prove_st_wf := 
       intro t; constructor; induction t; 
@@ -379,5 +161,5 @@ Module RED_REF_LANG_Help.
           destruct ec; inversion H; dep_subst; clear H
       ).
 
-End RED_REF_LANG_Help.
+End REF_LANG_Help.
 
