abstract_machine.v
@@ -1,3 +1,4 @@
+
 Module Type ABSTRACT_MACHINE.
 
   Parameters term configuration value : Set.
