reduction_strategy.v
@@ -1,0 +1,205 @@
+
+Module Type RED_STRATEGY_LANG.
+
+  Parameters term : Set.
+
+
+  Parameter elem_context : Set.
+  Parameter ckind        : Set. 
+  Parameter ckind_trans : ckind -> elem_context -> ckind.
+  Infix "+>" := ckind_trans (at level 50, left associativity).
+  Parameter  init_ckind : ckind.
+  Parameter  dead_ckind : ckind -> Prop.
+
+  Axiom death_propagation : 
+      forall k, dead_ckind k -> forall ec, dead_ckind (k+>ec).
+
+
+  Inductive context (k1 : ckind) : ckind -> Set :=
+  | empty : context k1 k1
+  | ccons : forall (ec : elem_context) {k2}, context k1 k2 -> context k1 (k2+>ec).
+  Arguments empty {k1}. Arguments ccons {k1} _ {k2} _.
+
+  Notation "[.]"      := empty.
+  Notation "[.]( k )" := (@empty k).
+  Infix    "=:"       := ccons (at level 60, right associativity).
+
+  Fixpoint compose {k1 k2} (c0 : context k1 k2) 
+                      {k3} (c1 : context k3 k1) : context k3 k2 := 
+      match c0 in context _ k2' return context k3 k2' with
+      | [.]     => c1
+      | ec=:c0' => ec =: compose c0' c1
+      end.
+  Infix "~+" := compose (at level 60, right associativity).
+
+  Parameter elem_plug : term -> elem_context -> term.
+  Notation "ec :[ t ]" := (elem_plug t ec) (at level 0).
+
+  Fixpoint plug (t : term) {k1 k2} (c : context k1 k2) : term :=
+      match c with
+      | [.]    => t 
+      | ec=:c' => plug ec:[t] c'
+      end.
+  Notation "c [ t ]" := (plug t c) (at level 0).
+
+  Axiom elem_plug_injective1 : forall ec {t0 t1}, ec:[t0] = ec:[t1] -> t0 = t1.
+
+
+  Definition immediate_ec ec t := exists t', ec:[t'] = t.
+
+
+  Parameters value redex : ckind -> Set.
+
+  Parameter value_to_term : forall {k}, value k -> term.
+  Coercion  value_to_term : value >-> term.
+  Parameter redex_to_term : forall {k}, redex k -> term.
+  Coercion  redex_to_term : redex >-> term.
+
+  Axiom value_to_term_injective : 
+      forall {k} (v v' : value k), value_to_term v = value_to_term v' -> v = v'.
+  Axiom redex_to_term_injective : 
+      forall {k} (r r' : redex k), redex_to_term r = redex_to_term r' -> r = r'.
+
+  Axiom proper_death : 
+      forall k, dead_ckind k -> ~ exists (r : redex k), True.
+
+
+
+  Axiom value_trivial1 : forall {k} (v : value k) ec {t}, 
+                             ~dead_ckind (k+>ec) -> ec:[t] = v -> 
+                                 exists (v' : value (k+>ec)), t = v'.
+  Axiom value_redex    : forall {k} (v : value k) (r : redex k), 
+                             value_to_term v <> redex_to_term r.
+
+
+  Inductive decomp k : Set :=
+  | d_red : forall {k'}, redex k' -> context k k' -> decomp k
+  | d_val : value k -> decomp k.
+  Arguments d_val {k} _. Arguments d_red {k} {k'} _ _.
+
+
+  Definition decomp_to_term {k} (d : decomp k) :=
+      match d with
+      | d_val v     => value_to_term v
+      | d_red _ r c => c[r]
+      end.
+  Coercion decomp_to_term : decomp >-> term.
+
+
+End RED_STRATEGY_LANG.
+
+
+
+
+Module Type RED_STRATEGY_STEP (R : RED_STRATEGY_LANG).
+
+  Import R.
+
+
+  (* interm_dec k - result of functions performing one step of decomposition of 
+                    a term t from the symbol k to a redex.
+     in_red r      - t is a redex, t = r.
+     in_term t' ec - t = ec[t'] and to find a redex we are going to check t'.
+     in_val v      - there is no redexes in t, t = v.
+     in_dead       - result of the functions for arguments out of their domains. *)
+  Inductive interm_dec k : Set :=
+  | in_red  : redex k -> interm_dec k
+  | in_term : term -> elem_context -> interm_dec k
+  | in_val  : value k -> interm_dec k
+  | in_dead : interm_dec k.
+  Arguments in_red {k} _.    Arguments in_val {k} _.
+  Arguments in_term {k} _ _. Arguments in_dead {k}.
+
+
+  (* dec_term t k       - one step of decomposition of t from the symbol k if we
+                          have no information about subterms of t. 
+                          Domain:  term * { k : ckind | k is not dead }  
+     dec_context ec k v - one step of decomposition of a term ec[t] with an additional
+                          piece of information saying that t is a value v. 
+                          Domain:  elem_context * { (k, v) | k+>ec is not dead and
+                                                             v : value (k+>ec)     }  *)
+  Parameter dec_term    : term -> forall k, interm_dec k.
+  Parameter dec_context : forall ec k, value (k+>ec) -> interm_dec k.
+
+
+  Axiom dec_term_correct : 
+      forall t k, match dec_term t k with
+      | in_red r      => t = r
+      | in_val v      => t = v
+      | in_term t' ec => t = ec:[t']
+      | in_dead       => dead_ckind k
+      end.
+
+  Axiom dec_term_from_dead : forall t k, 
+      dead_ckind k -> dec_term t k = in_dead.
+
+
+  Axiom dec_context_correct : 
+      forall ec k v, match dec_context ec k v with
+      | in_red r      => ec:[v] = r
+      | in_val v'     => ec:[v] = v'
+      | in_term t ec' => ec:[v] = ec':[t]
+      | in_dead       => dead_ckind (k+>ec) 
+      end.
+
+  Axiom dec_context_from_dead : forall ec k (v : value (k+>ec)), 
+      dead_ckind (k+>ec) -> dec_context ec k v = in_dead.
+
+
+  (* Any decomposition build by applying dec_term and dec_context needs to be proper. *)
+  Axiom dec_term_next_alive : forall t k {t0 ec0}, 
+      dec_term t k = in_term t0 ec0 -> ~ dead_ckind (k+>ec0).
+
+  Axiom dec_context_next_alive : forall ec k v {t0 ec0}, 
+      dec_context ec k v = in_term t0 ec0 -> ~ dead_ckind (k+>ec0).
+
+End RED_STRATEGY_STEP.
+
+
+
+
+Module Type RED_STRATEGY (R : RED_STRATEGY_LANG).
+
+  Import R.
+
+  Include RED_STRATEGY_STEP R.
+
+
+  Parameter search_order : ckind -> term -> elem_context -> elem_context -> Prop.
+  Notation "k , t |~  ec1 << ec2 " := (search_order k t ec1 ec2) 
+               (at level 70, t, ec1, ec2 at level 50, no associativity).
+
+
+  Axiom dec_term_red_atom : 
+      forall t k {r : redex k}, dec_term t k = in_red r -> 
+          ~exists ec, immediate_ec ec t /\ ~dead_ckind (k+>ec).
+
+  Axiom dec_term_val_atom : 
+      forall t k {v : value k}, dec_term t k = in_val v -> 
+          ~exists ec, immediate_ec ec t /\ ~dead_ckind (k+>ec).
+
+  Axiom dec_term_term_top : 
+      forall t k {t' ec}, dec_term t k = in_term t' ec -> 
+          forall ec',  ~ k, t |~ ec << ec'.
+
+
+  Axiom dec_context_red_bot : 
+      forall k ec v {r : redex k}, dec_context ec k v = in_red r -> 
+          forall ec',  ~ k, ec:[v] |~ ec' << ec.
+
+  Axiom dec_context_val_bot : 
+      forall k ec v {v' : value k}, dec_context ec k v = in_val v' -> 
+          forall ec',  ~ k, ec:[v] |~ ec' << ec.
+
+  Axiom dec_context_term_next : 
+      forall ec0 k v {t ec1}, dec_context ec0 k v = in_term t ec1 -> 
+      (*1*) k, ec0:[v] |~ ec1 << ec0 /\ 
+      (*2*) forall ec,  k, ec0:[v] |~ ec << ec0  ->  ~ k, ec0:[v] |~ ec1 << ec.
+
+
+  Axiom elem_context_det : 
+      forall t ec {t'}, t = ec:[t'] -> 
+          forall k ec',  k, t |~ ec' << ec -> 
+              exists (v : value (k+>ec)), t' = v.
+
+End RED_STRATEGY.
